FreydSSA/Body/Fun/Basic.lean
@@ -11,17 +11,17 @@ inductive UBody.FWf : Purity → FCtx ν (Ty α) → UBody φ ν → FCtx ν (Ty
   | let2 (x y) : e.FWf p Γ (Ty.pair A B) →
     FWf p ((Γ.cons x A).cons y B) t Δ → FWf p Γ (let2 x y e t) Δ
 
-def UBody.FWf.wk_entry {Γ' Γ Δ : FCtx ν (Ty α)} {t : UBody φ ν} (w: Γ'.Wk Γ)
+def UBody.FWf.wkEntry {Γ' Γ Δ : FCtx ν (Ty α)} {t : UBody φ ν} (w: Γ'.Wk Γ)
   : FWf p Γ t Δ → FWf p Γ' t Δ
   | nil _ w' => nil _ (w.comp w')
-  | let1 x de dt => let1 x (de.wk w) (dt.wk_entry (w.cons x _))
-  | let2 x y de dt => let2 x y (de.wk w) (dt.wk_entry ((w.cons x _).cons y _))
+  | let1 x de dt => let1 x (de.wk w) (dt.wkEntry (w.cons x _))
+  | let2 x y de dt => let2 x y (de.wk w) (dt.wkEntry ((w.cons x _).cons y _))
 
-def UBody.FWf.wk_exit {Γ Δ Δ' : FCtx ν (Ty α)} {t : UBody φ ν} (dt : FWf p Γ t Δ) (w: Δ.Wk Δ')
+def UBody.FWf.wkExit {Γ Δ Δ' : FCtx ν (Ty α)} {t : UBody φ ν} (dt : FWf p Γ t Δ) (w: Δ.Wk Δ')
   : FWf p Γ t Δ' := match dt with
   | nil _ w' => nil _ (w'.comp w)
-  | let1 x de dt => let1 x de (dt.wk_exit w)
-  | let2 x y de dt => let2 x y de (dt.wk_exit w)
+  | let1 x de dt => let1 x de (dt.wkExit w)
+  | let2 x y de dt => let2 x y de (dt.wkExit w)
 
 theorem UBody.FWf.allEq {Γ Δ : FCtx ν (Ty α)} {t : UBody φ ν} (dt : FWf p Γ t Δ) (dt' : FWf p Γ t Δ)
   : dt = dt' := by induction dt with
