FreydSSA/Body/Fun/Subst.lean
@@ -5,9 +5,14 @@ variable {φ ν α} [Φ : InstSet φ (Ty α)]
   [Φc : CohInstSet φ (Ty α)]
   [DecidableEq ν] [DecidableEq α]
 
-def UBody.FWf.subst {Γ' Γ Δ : FCtx ν (Ty α)} {t : UBody φ ν} {σ : USubst φ ν}
-  (hσ : Γ'.Subst σ Γ) (dt : t.FWf p Γ Δ)
-  : (Δ' : FCtx ν (Ty α)) × t.FWf p Γ' Δ' × Δ'.Subst (σ.cons_list t.defs) Δ
-  := sorry
+-- def UBody.FWf.subst {Γ' Γ Δ : FCtx ν (Ty α)} {t : UBody φ ν} {σ : USubst φ ν}
+--   (hσ : Γ'.Subst σ Γ) (dt : t.FWf p Γ Δ)
+--   : (Δ' : FCtx ν (Ty α)) × t.FWf p Γ' Δ' × Δ'.Subst (σ.cons_list t.defs) Δ
+--   := sorry
+
+-- def UBody.FWf.substEntry {Γ' Γ Δ : FCtx ν (Ty α)} {t : UBody φ ν} {σ : USubst φ ν}
+--   (hσ : Γ'.Subst σ Γ) (dt : t.FWf p Γ Δ) (hΔ : Δ.support ⊆ t.defs.toFinset)
+--   : t.FWf p Γ Δ
+--   := sorry
 
 --TODO: minimal UBody lore
