FreydSSA/Ctx/Label/Ix.lean
@@ -1,0 +1,19 @@
+import FreydSSA.Ctx.Label
+import FreydSSA.Ctx.Var.Ix
+
+variable {κ ν α} [DecidableEq κ] [DecidableEq ν] [DecidableEq α]
+
+--NOTE: ordering is κ ν α rather than ν κ α
+
+structure ILabel (κ : Type _) (ν : Type _) (α : Type _) where
+  name : κ
+  param : α
+  live : ICtx ν α
+
+structure ILCtx (κ : Type _) (ν : Type _) (α : Type _) : Type _ where
+  arity : ℕ
+  elements : Fin arity → ILabel κ ν α
+
+--TODO: as for ICtx, so ILCtx
+
+--TODO: functional ILCtx?
