FreydSSA/Ctx/Var/Ix.lean
@@ -1,0 +1,91 @@
+import FreydSSA.Ctx.Var
+import FreydSSA.Ctx.Var.Fun
+
+variable {ν ν' α β} [DecidableEq ν] [DecidableEq ν'] [DecidableEq α]
+
+structure TCtx (α : Type v) : Type _ where
+  arity : ℕ
+  ty : Fin arity → α
+
+structure ICtx (ν : Type u) (α : Type v) extends TCtx α : Type (max u v) where
+  name : Fin arity → ν
+
+structure IFCtx (ν : Type u) (α : Type v) extends ICtx (WithBot ν) α : Type (max u v) where
+  no_shadow : ∀ i j, name i = name j -> name i = ⊥ ∨ i = j
+
+structure ISCtx (ν : Type u) (α : Type v) extends ICtx ν α : Type (max u v) where
+  nodup : ∀ i j, name i = name j -> i = j
+
+structure FICtx (ν : Type u) (α : Type v) extends TCtx α : Type (max u v) where
+  ix : FCtx ν (Fin arity)
+  injective : Function.Injective ix
+
+--TODO: ICtx ≅ Ctx
+
+--TODO: map functions, positional map functions
+
+--TODO: ICtx → (IFCtx, FICtx)
+
+--TODO: FICtx ≅ IFCtx, TCtx equal...
+
+def TCtx.Var {α} (Γ : TCtx α) (A : α) (i : Fin Γ.arity) : Prop := Γ.ty i = A
+
+--TODO: factor out ix for Wk variants? can then use subset types...
+
+structure TCtx.Wk {α} (Γ : TCtx α) (Δ : TCtx α) (ρ : Fin Δ.arity → Fin Γ.arity) : Prop where
+  ty_eq : ∀i, Γ.ty (ρ i) = Δ.ty i
+  injective : Function.Injective ρ
+
+structure ICtx.Var {ν α} (Γ : ICtx ν α) (x : ν) (A : α) (i : Fin Γ.arity) : Prop where
+  ix_name : Γ.name i = x
+  ix_ty : Γ.ty i = A
+  ix_last : ∀j, Γ.name j = x → j ≤ i
+
+structure IFCtx.Var {ν α} (Γ : IFCtx ν α) (x : ν) (A : α) (i : Fin Γ.arity) : Prop where
+  ix_name : Γ.name i = x
+  ix_ty : Γ.ty i = A
+
+--TODO: IFCtx.Var ↔ ICtx.Var (using toICtx)
+
+structure FICtx.Var {ν α} (Γ : FICtx ν α) (x : ν) (A : α) (i : Fin Γ.arity) : Prop where
+  ix_name : Γ.ix x = i
+  ix_ty : Γ.ty i = A
+
+-- *syntactic* weakening, in which shadowed variables are simply ignored
+structure ICtx.VWk {ν α} (Γ : ICtx ν α) (Δ : ICtx ν α) where
+  ix : Fin Δ.arity → Fin Γ.arity
+  var : ∀{x A i}, Δ.Var x A i → Γ.Var x A (ix i)
+
+-- *semantic* weakening, which can be interpreted nicely for affine variables
+-- Note that the _names_ of shadowed variables don't matter
+structure ICtx.Wk {ν α} (Γ : ICtx ν α) (Δ : ICtx ν α) (ρ : Fin Δ.arity → Fin Γ.arity) extends TCtx.Wk Γ.toTCtx Δ.toTCtx ρ : Prop where
+  var : ∀{x A i}, Δ.Var x A i → Γ.Var x A (ρ i)
+
+--TODO: ICtx.Wk --> ICtx.VWk, with equal indices
+
+-- *strict* weakening, which does not swap variables, and respects all variable names
+structure ICtx.SWk {ν α} (Γ : ICtx ν α) (Δ : ICtx ν α) (ρ : Fin Δ.arity → Fin Γ.arity) extends Wk Γ Δ ρ : Prop where
+  name_eq : ∀i, Γ.name (ρ i) = Δ.name i
+  monotone : Monotone ρ
+
+--TODO: Strict weakning ≅ Ctx weakening
+
+--TODO: Weakening _preorder_ on ICtx
+
+--TODO: Connection between FCtx and ICtx
+
+
+--TODO: ICtx comparability
+
+structure IFCtx.VWk {ν α} (Γ : IFCtx ν α) (Δ : IFCtx ν α) (ρ : Fin Δ.arity → Fin Γ.arity) extends TCtx.Wk Γ.toTCtx Δ.toTCtx ρ : Prop where
+  var : ∀{x A i}, Δ.Var x A i → Γ.Var x A (ρ i)
+
+structure IFCtx.Wk {ν α} (Γ : IFCtx ν α) (Δ : IFCtx ν α) (ρ : Fin Δ.arity → Fin Γ.arity) extends TCtx.Wk Γ.toTCtx Δ.toTCtx ρ : Prop where
+  name_eq : ∀i, Γ.name (ρ i) = Δ.name i
+
+--TODO: IFCtx.Wk --> IFCtx.VWk
+
+structure FICtx.Wk {ν α} (Γ : FICtx ν α) (Δ : FICtx ν α) (ρ : Fin Δ.arity → Fin Γ.arity) extends TCtx.Wk Γ.toTCtx Δ.toTCtx ρ : Prop where
+  name_eq : ∀x, (Δ.ix x).map ρ ⊆ Γ.ix x
+
+--TODO: likewise for IFCtx, FICtx, ISCtx, etc...
